WIP

src/lowparse/LowParse.Spec.BitFields.fst
@@ -23,19 +23,46 @@ let rec bounds_of_widths (lo: nat) (hi: nat { lo <= hi }) (l: list nat) : Pure (
   | [_] -> []
   | sz :: q -> (lo + sz) :: bounds_of_widths (lo + sz) hi q
 
-let rec bitfields (tot: pos) (lo: nat) (hi: nat { lo <= hi /\ hi <= tot }) (l: list nat { valid_bitfield_widths lo hi l }) : Tot Type0 (decreases l) =
-  match l with
-  | [] -> unit
-  | [sz] -> BF.bitfield tot sz
-  | sz :: q -> BF.bitfield tot sz & bitfields tot (lo + sz) hi q
-
 module U = FStar.UInt
 
-let rec synth_bitfield (tot: pos) (lo: nat) (hi: nat { lo <= hi /\ hi <= tot }) (l: list nat { valid_bitfield_widths lo hi l }) (x: U.uint_t tot) : Tot (bitfields tot lo hi l) (decreases l) =
+inline_for_extraction
+noextract
+noeq
+type uint_t (tot: pos) (t: Type0) = {
+  v: (t -> Tot (U.uint_t tot));
+  uint_to_t: (U.uint_t tot -> Tot t);
+  v_uint_to_t: ((x: U.uint_t tot) -> Lemma (v (uint_to_t x) == x));
+  uint_to_t_v: ((x: t) -> Lemma (uint_to_t (v x) == x));
+  get_bitfield: ((x: t) -> (lo: nat) -> (hi: nat { lo <= hi /\ hi <= tot }) -> Tot (y: t { v y == BF.get_bitfield (v x) lo hi }));
+  set_bitfield: ((x: t) -> (lo: nat) -> (hi: nat { lo <= hi /\ hi <= tot }) -> (z: t { v z < pow2 (hi - lo) }) -> Tot (y : t { v y == BF.set_bitfield (v x) lo hi (v z)}));
+}
+
+let uint_t_v_uint_to_t #tot #t (cl: uint_t tot t) (x: U.uint_t tot) : Lemma
+  (cl.v (cl.uint_to_t x) == x)
+  [SMTPat (cl.v (cl.uint_to_t x))]
+= cl.v_uint_to_t x
+
+let uint_t_uint_to_t_v #tot #t (cl: uint_t tot t) (x: t) : Lemma
+  (cl.uint_to_t (cl.v x) == x)
+  [SMTPat (cl.uint_to_t (cl.v x))]
+= cl.uint_to_t_v x
+
+inline_for_extraction
+let bitfield (#tot: pos) (#t: Type0) (cl: uint_t tot t) (sz: nat { sz <= tot }) : Tot Type0 =
+  (x: t { cl.v x < pow2 sz })
+
+noextract
+let rec bitfields (#tot: pos) (#t: Type0) (cl: uint_t tot t) (lo: nat) (hi: nat { lo <= hi /\ hi <= tot }) (l: list nat { valid_bitfield_widths lo hi l }) : Tot Type0 (decreases l) =
+  match l with
+  | [] -> unit
+  | [sz] -> bitfield cl sz
+  | sz :: q -> bitfield cl sz & bitfields cl (lo + sz) hi q
+
+let rec synth_bitfield (#tot: pos) (#t: Type0) (cl: uint_t tot t) (lo: nat) (hi: nat { lo <= hi /\ hi <= tot }) (l: list nat { valid_bitfield_widths lo hi l }) (x: t) : Tot (bitfields cl lo hi l) (decreases l) =
   match l with
   | [] -> ()
-  | [_] -> BF.get_bitfield x lo hi
-  | sz :: q -> (BF.get_bitfield x lo (lo + sz), synth_bitfield tot (lo + sz) hi q x)
+  | [_] -> cl.get_bitfield x lo hi
+  | sz :: q -> (((cl.get_bitfield x lo (lo + sz) <: t) <: bitfield cl sz), synth_bitfield cl (lo + sz) hi q x)
 
 let rec synth_bitfield_injective (tot: pos) (lo: nat) (hi: nat { lo <= hi /\ hi <= tot }) (l: list nat { valid_bitfield_widths lo hi l }) (x y: U.uint_t tot) : Lemma
   (requires (synth_bitfield tot lo hi l x == synth_bitfield tot lo hi l y))
@@ -69,6 +96,54 @@ let rec synth_bitfield_ext (tot: pos) (lo: nat) (hi: nat { lo <= hi /\ hi <= tot
 #pop-options
 
 module U32 = FStar.UInt32
+module U64 = FStar.UInt64
+
+inline_for_extraction
+noextract
+let uint64 : uint_t 64 U64.t = {
+  v = U64.v;
+  uint_to_t = U64.uint_to_t;
+  v_uint_to_t = (fun _ -> ());
+  uint_to_t_v = (fun _ -> ());
+  get_bitfield = (fun x lo hi -> BF.get_bitfield64 x lo hi);
+  set_bitfield = (fun x lo hi z -> BF.set_bitfield64 x lo hi z);
+}
+
+inline_for_extraction
+noextract
+let uint32 : uint_t 32 U32.t = {
+  v = U32.v;
+  uint_to_t = U32.uint_to_t;
+  v_uint_to_t = (fun _ -> ());
+  uint_to_t_v = (fun _ -> ());
+  get_bitfield = (fun x lo hi -> BF.get_bitfield32 x lo hi);
+  set_bitfield = (fun x lo hi z -> BF.set_bitfield32 x lo hi z);
+}
+
+module U16 = FStar.UInt16
+module U8 = FStar.UInt8
+
+inline_for_extraction
+noextract
+let uint16 : uint_t 16 U16.t = {
+  v = U16.v;
+  uint_to_t = U16.uint_to_t;
+  v_uint_to_t = (fun _ -> ());
+  uint_to_t_v = (fun _ -> ());
+  get_bitfield = (fun x lo hi -> BF.get_bitfield16 x lo hi);
+  set_bitfield = (fun x lo hi z -> BF.set_bitfield16 x lo hi z);
+}
+
+inline_for_extraction
+noextract
+let uint8 : uint_t 8 U8.t = {
+  v = U8.v;
+  uint_to_t = U8.uint_to_t;
+  v_uint_to_t = (fun _ -> ());
+  uint_to_t_v = (fun _ -> ());
+  get_bitfield = (fun x lo hi -> BF.get_bitfield8 x lo hi);
+  set_bitfield = (fun x lo hi z -> BF.set_bitfield8 x lo hi z);
+}
 
 let synth_bitfield32 (l: list nat { valid_bitfield_widths 0 32 l }) (x: U32.t) : Tot (bitfields 32 0 32 l) =
   synth_bitfield 32 0 32 l (U32.v x)
