src/lowparse/LowParse.BitFields.fst
@@ -673,21 +673,35 @@ let bitfield_mask64 (lo: nat) (hi: nat { lo <= hi /\ hi <= 64 }) : Tot U64.t =
   normalize_term (U64.uint_to_t (bitfield_mask 64 lo hi))
 
 inline_for_extraction
+let u64_shift_right
+  (x: U64.t)
+  (amount: U32.t { U32.v amount <= 64 })
+: Tot (y: U64.t { U64.v y == U64.v x `U.shift_right` U32.v amount })
+= if amount = 64ul then 0uL else x `U64.shift_right` amount
+
+inline_for_extraction
 let get_bitfield64
-  (x: U64.t) (lo: nat { lo < 64 }) (hi: nat {lo <= hi /\ hi <= 64})
+  (x: U64.t) (lo: nat) (hi: nat {lo <= hi /\ hi <= 64})
 : Tot (y: U64.t { U64.v y == get_bitfield (U64.v x) lo hi })
-= (x `U64.logand` bitfield_mask64 lo hi) `U64.shift_right` (U32.uint_to_t lo)
+= (x `U64.logand` bitfield_mask64 lo hi) `u64_shift_right` (U32.uint_to_t lo)
 
 inline_for_extraction
 let not_bitfield_mask64 (lo: nat) (hi: nat { lo <= hi /\ hi <= 64 }) : Tot U64.t =
   normalize_term (U64.uint_to_t (not_bitfield_mask 64 lo hi))
 
 inline_for_extraction
+let u64_shift_left
+  (x: U64.t)
+  (amount: U32.t { U32.v amount <= 64 })
+: Tot (y: U64.t { U64.v y == U64.v x `U.shift_left` U32.v amount })
+= if amount = 64ul then 0uL else x `U64.shift_left` amount
+
+inline_for_extraction
 let set_bitfield64
-  (x: U64.t) (lo: nat { lo < 64 }) (hi: nat {lo <= hi /\ hi <= 64})
+  (x: U64.t) (lo: nat) (hi: nat {lo <= hi /\ hi <= 64})
   (v: U64.t { U64.v v < pow2 (hi - lo) })
 : Tot (y: U64.t { U64.v y == set_bitfield (U64.v x) lo hi (U64.v v) })
-= (x `U64.logand` not_bitfield_mask64 lo hi) `U64.logor` (v `U64.shift_left` U32.uint_to_t lo)
+= (x `U64.logand` not_bitfield_mask64 lo hi) `U64.logor` (v `u64_shift_left` U32.uint_to_t lo)
 
 (* Instantiate to UInt32 *)
 
@@ -696,21 +710,35 @@ let bitfield_mask32 (lo: nat) (hi: nat { lo <= hi /\ hi <= 32 }) : Tot U32.t =
   normalize_term (U32.uint_to_t (bitfield_mask 32 lo hi))
 
 inline_for_extraction
+let u32_shift_right
+  (x: U32.t)
+  (amount: U32.t { U32.v amount <= 32 })
+: Tot (y: U32.t { U32.v y == U32.v x `U.shift_right` U32.v amount })
+= if amount = 32ul then 0ul else x `U32.shift_right` amount
+
+inline_for_extraction
 let get_bitfield32
-  (x: U32.t) (lo: nat { lo < 32 }) (hi: nat {lo <= hi /\ hi <= 32})
+  (x: U32.t) (lo: nat) (hi: nat {lo <= hi /\ hi <= 32})
 : Tot (y: U32.t { U32.v y == get_bitfield (U32.v x) lo hi })
-= (x `U32.logand` bitfield_mask32 lo hi) `U32.shift_right` (U32.uint_to_t lo)
+= (x `U32.logand` bitfield_mask32 lo hi) `u32_shift_right` (U32.uint_to_t lo)
 
 inline_for_extraction
 let not_bitfield_mask32 (lo: nat) (hi: nat { lo <= hi /\ hi <= 32 }) : Tot U32.t =
   normalize_term (U32.uint_to_t (not_bitfield_mask 32 lo hi))
 
 inline_for_extraction
+let u32_shift_left
+  (x: U32.t)
+  (amount: U32.t { U32.v amount <= 32 })
+: Tot (y: U32.t { U32.v y == U32.v x `U.shift_left` U32.v amount })
+= if amount = 32ul then 0ul else x `U32.shift_left` amount
+
+inline_for_extraction
 let set_bitfield32
-  (x: U32.t) (lo: nat { lo < 32 }) (hi: nat {lo <= hi /\ hi <= 32})
+  (x: U32.t) (lo: nat) (hi: nat {lo <= hi /\ hi <= 32})
   (v: U32.t { U32.v v < pow2 (hi - lo) })
 : Tot (y: U32.t { U32.v y == set_bitfield (U32.v x) lo hi (U32.v v) })
-= (x `U32.logand` not_bitfield_mask32 lo hi) `U32.logor` (v `U32.shift_left` U32.uint_to_t lo)
+= (x `U32.logand` not_bitfield_mask32 lo hi) `U32.logor` (v `u32_shift_left` U32.uint_to_t lo)
 
 (* Instantiate to UInt16 *)
 module U16 = FStar.UInt16
@@ -720,21 +748,35 @@ let bitfield_mask16 (lo: nat) (hi: nat { lo <= hi /\ hi <= 16 }) : Tot U16.t =
   normalize_term (U16.uint_to_t (bitfield_mask 16 lo hi))
 
 inline_for_extraction
+let u16_shift_right
+  (x: U16.t)
+  (amount: U32.t { U32.v amount <= 16 })
+: Tot (y: U16.t { U16.v y == U16.v x `U.shift_right` U32.v amount })
+= if amount = 16ul then 0us else x `U16.shift_right` amount
+
+inline_for_extraction
 let get_bitfield16
-  (x: U16.t) (lo: nat { lo < 16 }) (hi: nat {lo <= hi /\ hi <= 16})
+  (x: U16.t) (lo: nat) (hi: nat {lo <= hi /\ hi <= 16})
 : Tot (y: U16.t { U16.v y == get_bitfield (U16.v x) lo hi })
-= (x `U16.logand` bitfield_mask16 lo hi) `U16.shift_right` (U32.uint_to_t lo)
+= (x `U16.logand` bitfield_mask16 lo hi) `u16_shift_right` (U32.uint_to_t lo)
 
 inline_for_extraction
 let not_bitfield_mask16 (lo: nat) (hi: nat { lo <= hi /\ hi <= 16 }) : Tot U16.t =
   normalize_term (U16.uint_to_t (not_bitfield_mask 16 lo hi))
 
 inline_for_extraction
+let u16_shift_left
+  (x: U16.t)
+  (amount: U32.t { U32.v amount <= 16 })
+: Tot (y: U16.t { U16.v y == U16.v x `U.shift_left` U32.v amount })
+= if amount = 16ul then 0us else x `U16.shift_left` amount
+
+inline_for_extraction
 let set_bitfield16
-  (x: U16.t) (lo: nat { lo < 16 }) (hi: nat {lo <= hi /\ hi <= 16})
+  (x: U16.t) (lo: nat) (hi: nat {lo <= hi /\ hi <= 16})
   (v: U16.t { U16.v v < pow2 (hi - lo) })
 : Tot (y: U16.t { U16.v y == set_bitfield (U16.v x) lo hi (U16.v v) })
-= (x `U16.logand` not_bitfield_mask16 lo hi) `U16.logor` (v `U16.shift_left` U32.uint_to_t lo)
+= (x `U16.logand` not_bitfield_mask16 lo hi) `U16.logor` (v `u16_shift_left` U32.uint_to_t lo)
 
 (* Instantiate to UInt8 *)
 module U8 = FStar.UInt8
@@ -744,18 +786,32 @@ let bitfield_mask8 (lo: nat) (hi: nat { lo <= hi /\ hi <= 8 }) : Tot U8.t =
   normalize_term (U8.uint_to_t (bitfield_mask 8 lo hi))
 
 inline_for_extraction
+let u8_shift_right
+  (x: U8.t)
+  (amount: U32.t { U32.v amount <= 8 })
+: Tot (y: U8.t { U8.v y == U8.v x `U.shift_right` U32.v amount })
+= if amount = 8ul then 0uy else x `U8.shift_right` amount
+
+inline_for_extraction
 let get_bitfield8
-  (x: U8.t) (lo: nat { lo < 8 }) (hi: nat {lo <= hi /\ hi <= 8})
+  (x: U8.t) (lo: nat) (hi: nat {lo <= hi /\ hi <= 8})
 : Tot (y: U8.t { U8.v y == get_bitfield (U8.v x) lo hi })
-= (x `U8.logand` bitfield_mask8 lo hi) `U8.shift_right` (U32.uint_to_t lo)
+= (x `U8.logand` bitfield_mask8 lo hi) `u8_shift_right` (U32.uint_to_t lo)
 
 inline_for_extraction
 let not_bitfield_mask8 (lo: nat) (hi: nat { lo <= hi /\ hi <= 8 }) : Tot U8.t =
   normalize_term (U8.uint_to_t (not_bitfield_mask 8 lo hi))
 
 inline_for_extraction
+let u8_shift_left
+  (x: U8.t)
+  (amount: U32.t { U32.v amount <= 8 })
+: Tot (y: U8.t { U8.v y == U8.v x `U.shift_left` U32.v amount })
+= if amount = 8ul then 0uy else x `U8.shift_left` amount
+
+inline_for_extraction
 let set_bitfield8
-  (x: U8.t) (lo: nat { lo < 8 }) (hi: nat {lo <= hi /\ hi <= 8})
+  (x: U8.t) (lo: nat) (hi: nat {lo <= hi /\ hi <= 8})
   (v: U8.t { U8.v v < pow2 (hi - lo) })
 : Tot (y: U8.t { U8.v y == set_bitfield (U8.v x) lo hi (U8.v v) })
-= (x `U8.logand` not_bitfield_mask8 lo hi) `U8.logor` (v `U8.shift_left` U32.uint_to_t lo)
+= (x `U8.logand` not_bitfield_mask8 lo hi) `U8.logor` (v `u8_shift_left` U32.uint_to_t lo)
